Make partiality more explicit in library functions of Lem shallow embedding
Some functions are partial, e.g. converting a bitvector to an integer, which
might fail for the bit list representation due to undefined bits.  Undefined
cases can be handled in different ways:

- call Lem's failwith, which maps to undefined/ARB in Isabelle and HOL (the
  default so far),
- return an option type,
- raise a failure  in the monad, or
- use a bitstream oracle to resolve undefined bits.

This patch adds different versions of partial functions corresponding to those
options.  The desired behaviour can be selected by choosing a binding in the
Sail prelude.  The naming scheme is that the failwith version is the default,
while the other versions have the suffixes _maybe, _fail, and _oracle,
respectively.

src/ast_util.ml
@@ -512,8 +512,8 @@ let string_of_base_effect_aux = function
   | BE_unspec -> "unspec"
   | BE_nondet -> "nondet"
   | BE_escape -> "escape"
-  | BE_lset -> "lset"
-  | BE_lret -> "lret"
+  (*| BE_lset -> "lset"
+  | BE_lret -> "lret"*)
 
 let string_of_base_kind_aux = function
   | BK_type -> "Type"
