src/pretty_print_common.ml
@@ -102,8 +102,8 @@ let doc_effect (BE_aux (e,_)) =
   | BE_wmem -> "wmem"
   | BE_wmv  -> "wmv"
   | BE_wmvt  -> "wmvt"
-  | BE_lset -> "lset"
-  | BE_lret -> "lret"
+  (*| BE_lset -> "lset"
+  | BE_lret -> "lret"*)
   | BE_eamem -> "eamem"
   | BE_exmem -> "exmem"
   | BE_barr -> "barr"
