lib/isabelle/Sail_values_lemmas.thy
@@ -2,6 +2,8 @@ theory Sail_values_lemmas
   imports Sail_values
 begin
 
+lemma nat_of_int_nat_simps[simp]: "nat_of_int = nat" by (auto simp: nat_of_int_def)
+
 termination reverse_endianness_list by (lexicographic_order simp add: drop_list_def)
 
 termination index_list
@@ -21,32 +23,67 @@ lemma just_list_cases:
         | (Some) ys where "xs = map Some ys" and "y = Some ys"
   using assms by (cases y) auto
 
-abbreviation "BC_bitU_list \<equiv> instance_Sail_values_Bitvector_list_dict instance_Sail_values_BitU_Sail_values_bitU_dict"
-lemmas BC_bitU_list_def = instance_Sail_values_Bitvector_list_dict_def instance_Sail_values_BitU_Sail_values_bitU_dict_def
-abbreviation "BC_mword \<equiv> instance_Sail_values_Bitvector_Machine_word_mword_dict"
-lemmas BC_mword_def = instance_Sail_values_Bitvector_Machine_word_mword_dict_def
+lemma bitops_bitU_of_bool[simp]:
+  "and_bit (bitU_of_bool x) (bitU_of_bool y) = bitU_of_bool (x \<and> y)"
+  "or_bit (bitU_of_bool x) (bitU_of_bool y) = bitU_of_bool (x \<or> y)"
+  "xor_bit (bitU_of_bool x) (bitU_of_bool y) = bitU_of_bool ((x \<or> y) \<and> \<not>(x \<and> y))"
+  "not_bit (bitU_of_bool x) = bitU_of_bool (\<not>x)"
+  "not_bit \<circ> bitU_of_bool = bitU_of_bool \<circ> Not"
+  by (auto simp: bitU_of_bool_def not_bit_def)
 
 lemma image_bitU_of_bool_B0_B1: "bitU_of_bool ` bs \<subseteq> {B0, B1}"
   by (auto simp: bitU_of_bool_def split: if_splits)
 
-lemma bool_of_bitU_bitU_of_bool[simp]: "bool_of_bitU \<circ> bitU_of_bool = id"
-  by (intro ext) (auto simp: bool_of_bitU_def bitU_of_bool_def)
+lemma bool_of_bitU_bitU_of_bool[simp]:
+  "bool_of_bitU \<circ> bitU_of_bool = Some"
+  "bool_of_bitU \<circ> (bitU_of_bool \<circ> f) = Some \<circ> f"
+  "bool_of_bitU (bitU_of_bool x) = Some x"
+  by (intro ext, auto simp: bool_of_bitU_def bitU_of_bool_def)+
+
+abbreviation "BC_bitU_list \<equiv> instance_Sail_values_Bitvector_list_dict instance_Sail_values_BitU_Sail_values_bitU_dict"
+lemmas BC_bitU_list_def = instance_Sail_values_Bitvector_list_dict_def instance_Sail_values_BitU_Sail_values_bitU_dict_def
+abbreviation "BC_mword \<equiv> instance_Sail_values_Bitvector_Machine_word_mword_dict"
+lemmas BC_mword_defs = instance_Sail_values_Bitvector_Machine_word_mword_dict_def
+  length_mword_def access_mword_def access_mword_inc_def access_mword_dec_def
+  (*update_mword_def update_mword_inc_def update_mword_dec_def*)
+  subrange_list_def subrange_list_inc_def subrange_list_dec_def
+  update_subrange_list_def update_subrange_list_inc_def update_subrange_list_dec_def
+
+lemma BC_mword_simps[simp]:
+  "unsigned_method BC_mword a = Some (uint a)"
+  "signed_method BC_mword a = Some (sint a)"
+  "length_method BC_mword (a :: ('a :: len) word) = int (LENGTH('a))"
+  by (auto simp: BC_mword_defs word_size)
 
 lemma nat_of_bits_aux_bl_to_bin_aux:
-  assumes "set bs \<subseteq> {B0, B1}"
-  shows "nat_of_bits_aux acc bs = nat (bl_to_bin_aux (map bool_of_bitU bs) (int acc))"
-  by (use assms in \<open>induction acc bs rule: nat_of_bits_aux.induct\<close>)
-     (auto simp: Bit_def bool_of_bitU_def intro!: arg_cong[where f = nat] arg_cong2[where f = bl_to_bin_aux])
+  "nat_of_bools_aux acc bs = nat (bl_to_bin_aux bs (int acc))"
+  by (induction acc bs rule: nat_of_bools_aux.induct)
+     (auto simp: Bit_def intro!: arg_cong[where f = nat] arg_cong2[where f = bl_to_bin_aux] split: if_splits)
 
-lemma nat_of_bits_bl_to_bin[simp]: "nat_of_bits (map bitU_of_bool bs) = nat (bl_to_bin bs)"
-  by (auto simp: nat_of_bits_def bl_to_bin_def nat_of_bits_aux_bl_to_bin_aux image_bitU_of_bool_B0_B1)
+lemma nat_of_bits_bl_to_bin[simp]: "nat_of_bools bs = nat (bl_to_bin bs)"
+  by (auto simp: nat_of_bools_def bl_to_bin_def nat_of_bits_aux_bl_to_bin_aux)
 
-lemma unsigned_bits_of_mword:
-  "unsigned_method BC_bitU_list (bits_of_method BC_mword a) = unsigned_method BC_mword a"
-  by (auto simp: BC_bitU_list_def BC_mword_def unsigned_of_bits_def)
+lemma unsigned_bits_of_mword[simp]:
+  "unsigned_method BC_bitU_list (bits_of_method BC_mword a) = Some (uint a)"
+  by (auto simp: BC_bitU_list_def BC_mword_defs unsigned_of_bits_def unsigned_of_bools_def)
 
-lemma unsigned_bits_of_bitU_list:
-  "unsigned_method BC_bitU_list (bits_of_method BC_bitU_list a) = unsigned_method BC_bitU_list a"
+lemma bits_of_bitU_list[simp]:
+  "bits_of_method BC_bitU_list v = v"
+  "of_bits_method BC_bitU_list v = Some v"
   by (auto simp: BC_bitU_list_def)
+
+lemma access_list_dec_rev_nth:
+  assumes "0 \<le> i" and "nat i < size xs"
+  shows "access_list_dec xs i = rev xs ! (nat i)"
+  using assms
+  by (auto simp: access_list_dec_def access_list_inc_def length_list_def rev_nth
+           intro!: arg_cong2[where f = List.nth])
+
+lemma access_bv_dec_mword[simp]:
+  fixes w :: "('a::len) word"
+  assumes "0 \<le> n" and "nat n < LENGTH('a)"
+  shows "access_bv_dec BC_mword w n = bitU_of_bool (w !! (nat n))"
+  using assms
+  by (auto simp: access_bv_dec_def access_list_def access_list_dec_rev_nth BC_mword_defs rev_map test_bit_bl word_size)
 
 end
